VisualProof/Rule/WirePrimitive.lean
@@ -5,6 +5,7 @@ import VisualProof.Rule.WirePrimitive.Arguments
 import VisualProof.Rule.WirePrimitive.ArgumentsDropTransport
 import VisualProof.Rule.WirePrimitive.ArgumentsExtendTransport
 import VisualProof.Rule.WirePrimitive.ArgumentsArityTransport
+import VisualProof.Rule.WirePrimitive.ArgumentsDuplicateTransport
 import VisualProof.Rule.WirePrimitive.Leaves
 import VisualProof.Rule.WirePrimitive.Program
 
